progress with syntax

Veil/DSL/ActionLang.lean
@@ -14,27 +14,11 @@ open Lean Elab Command Term Meta Lean.Parser
   This file defines the syntax and semantics for the imperative language
   we use to define initializers and actions.
 -/
-section Lang
+section Veil
+
+section Types
 /-! Our language is parametric over the state type. -/
 variable (σ : Type)
-
-/-- Imperative language for defining actions. -/
-inductive Lang.{u} : Type u → Type (u + 1) where
-  /-- Pre-condition. All capital variables will be quantified. -/
-  | require (rq : σ -> Prop) : Lang PUnit
-  | bind    {ρ ρ' : Type u} (act : Lang ρ') (act' : ρ' -> Lang ρ) : Lang ρ
-  -- τ is a first order type, so it can be quantified in FOL
-  | fresh   (τ : Type u) : Lang τ
-  /-- Deterministic changes to the state, although mostly used for assignments. All
-      capital variables will be quantified. -/
-  | det     {ρ' : Type u} (act : σ -> σ × ρ') : Lang ρ'
-  /-- Non-deterministic changes to the state. -/
-  | nondet  {ρ' : Type u} (act :  σ -> σ × ρ' -> Prop) : Lang ρ'
-  /-- If-then-else. `open Classical` to allow propositions in the condition. -/
-  | ite     {ρ : Type u} (cnd : σ -> Bool) (thn : Lang ρ) (els : Lang ρ) : Lang ρ
-  /-- If-then-else. `open Classical` to allow propositions in the condition. -/
-  | iteSome {ρ : Type u} {ρ' : Type} (cnd : ρ' -> σ -> Bool) (thn : ρ' -> Lang ρ) (els : Lang ρ) : Lang ρ
-  | ret     {ρ : Type u} (ret : ρ) : Lang ρ
 
 /-- One-state formula -/
 @[inline] abbrev sprop := σ -> Prop
@@ -43,222 +27,64 @@ inductive Lang.{u} : Type u → Type (u + 1) where
 /-- Two-state formula -/
 @[inline] abbrev actprop := σ -> σ -> Prop
 
-
 def Wlp (σ : Type) (ρ : Type) := rprop σ ρ -> sprop σ
 
+end Types
 section
 
 variable {σ ρ : Type}
 
-def Wlp.pure {σ ρ} (r : ρ) : Wlp σ ρ := fun post s => post r s
-def Wlp.bind {σ ρ} (wp : Wlp σ ρ) (wp_cont : ρ -> Wlp σ ρ') : Wlp σ ρ' :=
+@[actSimp]
+def Wlp.pure (r : ρ) : Wlp σ ρ := fun post => post r
+@[actSimp]
+def Wlp.bind (wp : Wlp σ ρ) (wp_cont : ρ -> Wlp σ ρ') : Wlp σ ρ' :=
   fun post s => wp (fun r s' => wp_cont r post s') s
 
 instance : Monad (Wlp σ) where
   pure := Wlp.pure
   bind := Wlp.bind
 
+@[actSimp]
 def Wlp.require (rq : sprop σ) : Wlp σ PUnit := fun post s => rq s ∧ post () s
-def Wlp.det (act : σ -> σ × ρ) : Wlp σ ρ := fun post s => let (s', ret) := act s ; post ret s'
-def Wlp.nondet (act : σ -> σ × ρ -> Prop) : Wlp σ ρ := fun post s => ∃ s' ret, act s (s', ret) ∧ post ret s'
+@[actSimp]
+def Wlp.det (act : σ -> ρ × σ) : Wlp σ ρ := fun post s => let (ret, s') := act s ; post ret s'
+@[actSimp]
+def Wlp.nondet (act : σ -> ρ × σ -> Prop) : Wlp σ ρ := fun post s => ∃ s' ret, act s (ret, s') ∧ post ret s'
+@[actSimp]
 def Wlp.ite (cnd : σ -> Bool) (thn : Wlp σ ρ) (els : Wlp σ ρ) : Wlp σ ρ :=
   fun post s => if cnd s then thn post s else els post s
-def Wlp.iteSome (cnd : ρ -> σ -> Bool) (thn : ρ -> Wlp σ ρ) (els : Wlp σ ρ) : Wlp σ ρ :=
+@[actSimp]
+def Wlp.iteSome (cnd : ρ -> σ -> Bool) (thn : ρ -> Wlp σ ρ') (els : Wlp σ ρ') : Wlp σ ρ' :=
   fun post s => (∃ r, cnd r s ∧ thn r post s) ∨ (∀ r, ¬ cnd r s) ∧ els post s
+@[actSimp]
 def Wlp.fresh (τ : Type) : Wlp σ τ := fun post s => ∃ t, post t s
+@[actSimp]
 def Wlp.skip : Wlp σ PUnit := Wlp.pure ()
+@[actSimp]
+def Wlp.withState {σ} (r : σ -> ρ) : Wlp σ ρ :=
+  fun post s => post (r s) s
 
-partial def getCapitals (s : Syntax) :=
-  let rec loop  (acc : Array $ TSyntax `ident ) (s : Syntax) : Array $ TSyntax `ident :=
-    if s.isIdent then
-      if isCapital s then
-        acc.push ⟨s⟩
-      else
-        acc
-    else
-      s.getArgs.foldl (init := acc) loop
-  (loop #[] s).toList.eraseDups.toArray
-
-/-- Close the given expression under all capital letters.
-    this is called for `require`, `safety` and `invariant` -/
-def closeCapitals (s : Term) : MacroM Term :=
-  let caps := getCapitals s
-  `(forall $[$caps]*, $s)
-
-/-- Throw an error if the field (which we're trying to assign to) was
-declared immutable. FIXME: make sure elaboration aborts? -/
-def throwIfImmutable (lhs : TSyntax `Lean.Parser.Term.structInstLVal) : TermElabM Unit := do
-  let spec := (← localSpecCtx.get).spec
-  let nm ← getIdFrom lhs
-  let .some comp := spec.getStateComponent nm
-    | throwErrorAt lhs "trying to assign to undeclared state component {nm}"
-  if comp.isImmutable then
-    throwErrorAt lhs "{comp.kind} {comp.name} was declared immutable, but trying to assign to it!"
-  where getIdFrom (lhs : TSyntax `Lean.Parser.Term.structInstLVal) : TermElabM Name :=
-    match lhs with
-    | `(Lean.Parser.Term.structInstLVal|$id:ident) => pure id.getId
-    | _ => throwErrorAt lhs "expected an identifier in the LHS of an assignment, got {repr lhs}"
-
-/-- This is used in `require` were we define a predicate over a state.
-    Instead of writing `fun st => Pred` this command will pattern match over
-    `st` making all its fields accessible for `Pred` -/
-macro "funcases" t:term : term => `(term| by intros st; unhygienic cases st; exact $t)
-macro "funcases" id:ident t:term : term => `(term| by unhygienic cases $id:ident; exact $t)
-
-/-- `require s` checks if `s` is true on the current state -/
-syntax "require" term      : doElem
-/-- `call s` calls action `s` on a current state -/
-syntax "call" term : doElem
-
-/-- Non-deterministic value. -/
-syntax (name := nondetVal) "*" : term
-/-- syntax for assigment, e.g. `pending n s := true` -/
-syntax atomic(Term.structInstLVal (term:max)* ":==") (term <|> nondetVal)    : doElem
-
-elab "throw_if_immutable" id:Term.structInstLVal t:term : term => do
-  throwIfImmutable id; elabTerm t none
-
-macro_rules
-  | `(doElem| require $t)           => `(doElem| Wlp.require (funcases $t))
-  | `(doElem| call $t)              => `(doElem| @Wlp.nondet _ _ (funcases $t))
-  -- expansion of the intermediate syntax for assigment
-  -- for instance `pending := pending[n, s ↦ true]` will get
-  -- expanded to `Lang.det (fun st => { st with pending := st.pending[n, s ↦ true] })`
-  | `(doElem| $id:structInstLVal :== $t:term) =>
-    `(doElem|
-            /- TODO: uncomment -/
-            -- throw_if_immutable $id
-            @Wlp.det _ _ (fun st => ({ st with $id := (funcases st $t)}, ())))
-  -- expansion of the actual syntax for assignment
-  -- for instance `pending n s := true` will get
-  -- expanded to `pending := pending[n, s ↦ true]`
-  | `(doElem| $id:structInstLVal $ts: term * :== $t:term) => do
-    let stx <- withRef id `($(⟨id.raw.getHead?.get!⟩)[ $[$ts],* ↦ $t:term ])
-    `(doElem| $id:structInstLVal :== $stx)
+macro "unfold_wlp" : conv =>
+  `(conv| unfold
+    Wlp.det
+    Wlp.pure
+    Wlp.bind
+    Wlp.require
+    Wlp.ite
+    Wlp.iteSome
+    Wlp.fresh
+    Wlp.skip
+    Wlp.withState
+    Wlp.nondet)
 
 
-elab_rules : term
-  -- expansion of the intermediate syntax for assigment
-  -- for instance `pending := pending[n, s ↦ true]` will get
-  -- expanded to `Lang.det (fun st => { st with pending := st.pending[n, s ↦ true] })`
-  | `(doElem| $id:structInstLVal :== $t:term) => do
-    throwIfImmutable id
-    elabTerm (<- `(doElem|@Wlp.det _ _ (fun (st : [State]) =>
-      ({ st with $id := (funcases st $t)}, ())))) none
-  -- expansion of the actual syntax for assignment
-  -- for instance `pending n s := true` will get
-  -- expanded to `pending := pending[n, s ↦ true]`
-
-
-structure state where
-  r : Int
-  s : Bool
-  m : Bool -> Bool
-
-
-open Wlp in
-def k : Wlp state Nat := do
-  let mut y := 0
-  require r = y
-  if true then
-    y := (<- fresh Nat) + 1
-  else y := y + 2
-  m B :== true
-  return y
-
-example {P : _ -> Prop} : P (k (fun r s => r = r' ∧ s = s') s) := by
-  simp [k, Wlp.fresh, bind, Wlp.bind, Wlp.require, pure, Wlp.pure, Wlp.det ]
-
-
-
-
-
-
+instance : MonadStateOf σ (Wlp σ) where
+  get := fun post s => post s s
+  set s' := fun post _ => post () s'
+  modifyGet := Wlp.det
 
 end
 
-#exit
--- abbrev triple (t : ρ) (H : sprop σ) (P : rprop σ ρ) := ∀ s, H s → P t s
-
-/-- Weakest liberal precondition transformer. It takes a post-condition and
-    a program and returns the weakest pre-condition that guarantees the
-    post-condition IF the program terminates.
-    This defines the axiomatic semantics of our language. -/
-@[actSimp] def wlp (post : rprop σ ρ) : Lang σ ρ -> sprop σ
-  -- `require` enhances the pre-condition, restricting the possible states
-  -- it has the same effect as `assume` in Hoare logic
-  | Lang.require rq       => fun s => rq s ∧ post () s
-  -- | Lang.assume  as       => fun s => as s → post () s
-  -- a deterministic `act` transforms the state
-  | Lang.det act          => fun s => let (s', ret) := act s ; post ret s'
-  -- A non-deterministic action satisfies the post-condition if there is
-  -- _some_ possible post-state that satisfies the post-condition.
-  -- This corresponds to the semantics in Ivy and matches the intuition that
-  -- a call to an action is morally equivalent to inlining that action.
-  | Lang.nondet act       => fun s => ∃ s' ret, act s (s', ret) ∧ post ret s'
-  -- the meaning of `ite` depends on which branch is taken
-  | Lang.ite cnd thn els  => fun s => if cnd s then wlp post thn s else wlp post els s
-  | Lang.iteSome cnd thn els  =>
-    fun s =>
-    (∃ r, cnd r s ∧ wlp post (thn r) s) ∨ (∀ r, ¬ cnd r s) ∧ wlp post els s
-  -- `seq` is a composition of programs, so we need to compute the wlp of
-  -- the first program, given the wlp of the second
-  | Lang.ret ret    => post ret
-  | Lang.bind l1 l2 => wlp (fun ret => wlp post (l2 ret)) l1
-  | Lang.fresh τ => fun s => ∃ t, post t s
-
-declare_syntax_cat left_arrow
-syntax "<-" : left_arrow
-syntax "←" : left_arrow
-
-/-- Sequense of [lang] commands -/
-declare_syntax_cat langSeq
-/-- Let binding or a single [lang] statement -/
-declare_syntax_cat langElem
-/-- Single [lang] statement -/
-declare_syntax_cat lang
-
-syntax lang : langElem
-/- [lang] let binging -/
-syntax "let" ident left_arrow lang : langElem
-
-/-- Sequense of [lang] commands -/
-syntax sepByIndentSemicolon(langElem) : langSeq
-
-/-- [skip] statement which does nothing -/
-syntax "skip"              : lang
-/-- Non-deterministic value. -/
-syntax (name := nondetVal) "*" : lang
-/-- `require s` checks if `s` is true on the current state -/
-syntax "require" term      : lang
-/-- `fresh [Type]?` creates a fresh variable of type `Type`, or of an implicit type if `Type` is ommited -/
-syntax "fresh" term ? : lang
-/-- `return t` returns `t`  -/
-syntax "return" term : lang
-syntax term : lang
-
-declare_syntax_cat some_if
-syntax ident "where" : some_if
-syntax (priority := high) "if " (some_if)? term " then" langSeq colGe "else\n" langSeq : lang
-syntax (priority := low) "if " (some_if)? term " then" langSeq : lang
-
-/-- intermediate syntax for assigment, e.g. `pending := pending[n, s ↦ true]` -/
-syntax Term.structInstLVal ":=" term    : lang
-/-- syntax for assigment, e.g. `pending n s := true` -/
-syntax Term.structInstLVal (term:max)+ ":=" (term <|> nondetVal)    : lang
-syntax term (":" term)? left_arrow lang "in" langSeq : lang
-
-declare_syntax_cat unchanged
-syntax "with unchanged" "[" ident,* "]" : unchanged
-syntax "ensure" rcasesPat  "," term unchanged ? : lang
-syntax "ensure" term unchanged ? : lang
-syntax "[unchanged|" ident* "]" : term
-
-/-- Syntax to trigger the expantion into a code -/
-syntax "[langSeq|" langSeq "]" : term
-syntax "[lang|" lang "]" : term
-
-
 partial def getCapitals (s : Syntax) :=
   let rec loop  (acc : Array $ TSyntax `ident ) (s : Syntax) : Array $ TSyntax `ident :=
     if s.isIdent then
@@ -290,95 +116,98 @@ def throwIfImmutable (lhs : TSyntax `Lean.Parser.Term.structInstLVal) : TermElab
     | `(Lean.Parser.Term.structInstLVal|$id:ident) => pure id.getId
     | _ => throwErrorAt lhs "expected an identifier in the LHS of an assignment, got {repr lhs}"
 
-/-- This is used in `require` were we define a predicate over a state.
-    Instead of writing `fun st => Pred` this command will pattern match over
-    `st` making all its fields accessible for `Pred` -/
-macro "funcases" t:term : term => `(term| by intros st; unhygienic cases st; exact $t)
-macro "funcases" id:ident t:term : term => `(term| by unhygienic cases $id:ident; exact $t)
-
-/-====== Macro expansion for [lang] ======-/
+def getFields : TermElabM (Array Name) := do
+  let spec := (← localSpecCtx.get).spec
+  pure $ spec.signature.map (·.name)
 
 /-- In some cases, during the macro expansion, we need to annotate certain
     arguments with the state type. To get the state type, we need an access to an
     eviorment with we don't have at the macro-expansion stage. To overcome this, we
     introduce the following notation, witch gets resolved to a current state type
     during the elaboration stage  -/
-syntax "[State]" : term
-elab_rules : term
-  | `([State]) => do
+elab "[State]" : term => do
     let stateTp := (← localSpecCtx.get).spec.stateStx
     elabTerm (<- `(term| $stateTp)) none
 
-/- Fisrt, we handle sequensial composiotin and let-bindings -/
+/-- This is used in `require` were we define a predicate over a state.
+    Instead of writing `fun st => Pred` this command will pattern match over
+    `st` making all its fields accessible for `Pred` -/
+macro "funcases" t:term : term => `(term| by intros st; unhygienic cases st; exact $t)
+macro "funcases" id:ident t:term : term => `(term| by unhygienic cases $id:ident; exact $t)
+
+/-- `require s` checks if `s` is true on the current state -/
+syntax "require" term      : term
+/-- `call s` calls action `s` on a current state -/
+syntax "call" term : term
+/-- `fresh [ty]?` allocate a fresh variable of a given type `ty` -/
+syntax "fresh" term ? : term
+
+/-- Non-deterministic value. -/
+syntax (name := nondetVal) "*" : term
+
+declare_syntax_cat doSeqVeil
+declare_syntax_cat doElemVeil
+
+syntax (priority := low) doElem : doElemVeil
+
+syntax "if" term "then" doSeqVeil colGe "else" doSeqVeil : doElemVeil
+syntax "if" term "then" doSeqVeil : doElemVeil
+syntax "if" ident ":" term "then" doSeqVeil colGe "else" doSeqVeil : doElemVeil
+syntax "if" ident ":" term "then" doSeqVeil : doElemVeil
+
+
+declare_syntax_cat unchanged
+syntax "with unchanged" "[" ident,* "]" : unchanged
+syntax "ensure" rcasesPat  "," term unchanged ? : term
+syntax "ensure" term unchanged ? : term
+syntax "[unchanged|" ident* "]" : term
+
+syntax sepByIndentSemicolon(doElemVeil) : doSeqVeil
+
+mutual
+partial def expandDoSeqVeil (stx : TSyntax `doSeqVeil) : TermElabM (TSyntax ``Term.doSeq) :=
+  match stx with
+  | `(doSeqVeil| $doS:doElemVeil*) => do
+    let doS <- doS.getElems.mapM expandDoElemVeil
+    `(doSeq| $[$doS:doElem]*)
+  | _ => throwErrorAt stx s!"unexpected syntax of Veil `do`-notation sequence {stx}"
+
+partial def expandDoElemVeil (stx : TSyntax `doElemVeil) : TermElabM (TSyntax `doElem) :=
+  match stx with
+  | `(doElemVeil| if $t:term then $thn:doSeqVeil else $els:doSeqVeil) => do
+    let thn <- expandDoSeqVeil thn
+    let els <- expandDoSeqVeil els
+    `(doElem| if <- Wlp.withState (funcases $t) then $thn else $els)
+  | `(doElemVeil| if $t:term then $thn:doSeqVeil) => do
+    expandDoElemVeil $ <- `(doElemVeil| if $t then $thn:doSeqVeil else pure ())
+  | `(doElemVeil| $doE:doElem) =>
+    match doE with
+    | `(doElem| $id:ident := $t:term) => do
+        let id' <- `(Term.structInstLVal| $id:ident)
+        let fields <- getFields
+        if id.getId ∈ fields then
+          throwIfImmutable id'
+          `(doElem| @Wlp.det _ _ (fun (st : [State]) => ((), { st with $id' := (funcases st $t)})))
+        else
+          `(doElem| $id:ident := $t:term)
+    | `(doElem| $idts:term := $t:term) => do
+      let some (id, ts) := idts.isApp? | `(doElem| $doE:doElem)
+      let stx <- withRef idts `(term| $id[ $[$ts],* ↦ $t:term ])
+      let stx <- `(doElemVeil| $id:ident := $stx)
+      expandDoElemVeil stx
+    | _ => `(doElem| $doE:doElem)
+  | _ => throwErrorAt stx s!"unexpected syntax of Veil `do`-notation {stx}"
+end
+
+elab "do'" stx:doSeqVeil : term => do
+  let stx <- expandDoSeqVeil stx
+  elabTerm (<- `(term| ((do $stx) : Wlp [State] _))) none
 
 macro_rules
-  | `([langSeq| ]) => `([lang|skip])
-  | `([lang|skip]) => do
-    `(term| @Lang.det _ _ (fun (st : [State]) => (st, ())))
-  | `([langSeq|$l:lang]) => `([lang|$l])
-  | `([langSeq| $ls:langElem*]) => do
-    let l₁ := ls.getElems[0]!
-    let ls := ls.getElems[1:]
-    let mut (id, l) := (default, default)
-    match l₁ with
-    | `(langElem| let $i:ident $_:left_arrow $lb:lang) =>
-      id <- `(Term.funBinder| $i); l := lb
-    | `(langElem| $lb:lang) =>
-      id <- `(Term.funBinder| _); l := lb
-    | _ => Macro.throwError "unexpected syntax"
-    `(@Lang.bind _ _ _ [lang|$l] (fun $id => [langSeq|$[$ls]*]))
-
-
-/- Simple single statements: `require`, `return`, `fresh` and `call` -/
-
-macro_rules
-  | `([lang|return $t:term]) => `(@Lang.ret _ _ (funcases $(mkIdent `st):ident $t))
-  | `([lang|$t:term])   => `(@Lang.nondet _ _ (funcases $(mkIdent `st):ident $t))
-  | `([lang|require $t:term]) => do
-    -- universally close term [t] under free variables starting with a capital letter
-    let t' <- closeCapitals t
-    withRef t $ `(@Lang.require _ (funcases ($t' : Prop) : _ -> Prop))
-    -- infer the type of a fresh variable, if it is not given
-  | `([lang|fresh]) => `([lang|fresh _])
-  | `([lang|fresh $t:term]) => `(@Lang.fresh _ $t)
-
-/- If-then-else -/
-
-macro_rules
-  | `([lang|if $some_if ? $cnd:term then $thn:langSeq]) => `([lang|if $some_if ? $cnd then $thn else skip])
-  | `([lang|if $cnd:term then $thn:langSeq else $els:langSeq]) => do
-    let cnd' <- closeCapitals cnd
-    -- condition might depend on the state as well
-    let cnd <- withRef cnd `(funcases ($cnd' : Bool))
-    `(@Lang.ite _ _ ($cnd: term) [langSeq|$thn] [langSeq|$els])
-  | `([lang|if $x:ident where $cnd:term then $thn:langSeq else $els:langSeq]) => do
-    let cnd' <- closeCapitals cnd
-    -- condition might depend on the state as well
-    let cnd <- withRef cnd `(funcases ($cnd' : Bool))
-    `(@Lang.iteSome _ _ _ (fun $x:ident => $cnd:term) (fun $x => [langSeq|$thn]) [langSeq|$els])
-
-/- Assignments -/
-
-elab_rules : term
-  -- expansion of the intermediate syntax for assigment
-  -- for instance `pending := pending[n, s ↦ true]` will get
-  -- expanded to `Lang.det (fun st => { st with pending := st.pending[n, s ↦ true] })`
-  | `([lang| $id:structInstLVal := $t:term]) => do
-    throwIfImmutable id
-    elabTerm (<- `(@Lang.det _ _ (fun (st : [State]) =>
-      ({ st with $id := (funcases st $t)}, ())))) none
-  -- non-deterministic assignment
-  | `([lang| $id:structInstLVal $ts: term * := *]) => do
-    throwIfImmutable id
-    elabTerm (<- `(@Lang.fresh _ _ _ (fun v => @Lang.nondet _ _ _ (fun (st : [State]) =>
-      ({ st with $id := (funcases st ($(⟨id.raw.getHead?.get!⟩)[ $[$ts],* ↦ v ]))}, ()))))) none
-  -- expansion of the actual syntax for assignment
-  -- for instance `pending n s := true` will get
-  -- expanded to `pending := pending[n, s ↦ true]`
-  | `([lang| $id:structInstLVal $ts: term * := $t:term]) => do
-    throwIfImmutable id
-    let stx <- withRef id `($(⟨id.raw.getHead?.get!⟩)[ $[$ts],* ↦ $t:term ])
-    elabTerm (<- `([lang| $id:structInstLVal := $stx])) none
+  | `(require $t) => `(Wlp.require (funcases $t))
+  | `(call    $t) => `(Wlp.nondet (funcases $t))
+  | `(fresh   $t) => `(Wlp.fresh $t)
+  | `(fresh)      => `(Wlp.fresh _)
 
 /- Ensures statement -/
 
@@ -398,7 +227,7 @@ elab "with_rename_old" t:tactic : tactic => withMainContext do
           let new_name := String.intercalate "_" nms.dropLast ++ "_old" |>.toName
           evalTactic $ <- `(tactic| (revert $(mkIdent hyp.userName):ident; intros $(mkIdent new_name):ident))
 
-/- Expanding unchanged statement -/
+/- Expanding `unchanged` statement -/
 macro_rules
   | `([unchanged| $id:ident]) =>
     let id_old := id.getId.toString ++ "_old" |>.toName
@@ -408,26 +237,28 @@ macro_rules
 
 /- One can omit the result variable from [ensures] -/
 macro_rules
-  | `([lang|ensure $t:term $un:unchanged ?] ) => `([lang|ensure (_ : Unit), $t:term $un:unchanged ?])
+  | `(ensure $t:term $un:unchanged ?) => `(ensure (_ : Unit), $t:term $un:unchanged ?)
 
 elab_rules : term
   /- if the list of unchanged state fileds is omitted, we can restore it by
      checking witch of them are mentioned in the [ensures] body. By default
      we assume that if the state filed is not mentioned, then it is left
      unchanged  -/
-  | `([lang|ensure $r, $t:term]) => do
-    let fields : Array Name := (<- localSpecCtx.get).spec.signature.map (·.name)
+  | `(ensure $r, $t:term) => do
+    let fields : Array Name <- getFields
     let mut unchangedFields := #[]
     for f in fields do
       unless t.raw.find? (·.getId == f) |>.isSome do
         unchangedFields := unchangedFields.push $ mkIdent f
-    elabTerm (<- `(term| [lang|ensure $r, $t:term with unchanged[$[$unchangedFields],*]])) none
-  | `([lang|ensure $r, $t:term with unchanged[$ids,*]]) => do
+    elabTerm (<- `(ensure $r, $t:term with unchanged[$[$unchangedFields],*])) none
+  | `(ensure $r, $t:term with unchanged[$ids,*]) => do
     withRef t $
-    elabTerm (<- `(term| @Lang.nondet _ _ (
+    elabTerm (<- `(term| @Wlp.nondet _ _ (
       by rintro st ⟨st', $r⟩;
          unhygienic cases st';
          with_rename_old unhygienic cases st;
          exact $t ∧ [unchanged|$ids*]))) none
 
-end Lang
+attribute [actSimp] Bind.bind Pure.pure
+
+end Veil
