Test/Syntax.lean
@@ -2,45 +2,41 @@ import Veil.DSL
 
 section Test
 
+open Classical
+
 type node
 
-relation r : node -> node -> Prop
+relation r : node -> Nat -> Prop
+individual n : node
 
 #gen_state Test
 
-#check
-   if true then
-      true
-    else false
 
 action foo (k : Nat) = {
-  skip
-  skip; skip
-  let x <- skip
-  require x = x
-  let y <- return 5
-  require y = 5
-  return 5
-  let x <- require y = 5
-  require x = ()
-  let x <- fresh Int
-  require x = k
-  let x <- fresh
-  require x = ()
-  if (x = ()) then
-    skip
+  let x <- fresh node
+  require r x k
+}
+
+action foo2 (k : Nat) = {
+  let mut y := 0
+  y := k
+  if y > 0 then
+    return true
+  else return false
+  -- r N k := True
+}
+
+action foo3 (k : Nat) = {
+  let x <- fresh node
+  n := x
+  let mut y := 0
+  if r x k then
+    r x k := True
+    y := 0
   else
-    skip
-  -- else return 5
+    y := 1
+  return y
 }
-
-action bar = {
-  !foo 5
-  r N M := True
-  let m <- fresh
-  ensure r m m = False
-}
-
 
 
 end Test
