Veil/DSL/Tactic.lean
@@ -1,6 +1,7 @@
 import Lean.Elab.Tactic
 import Veil.DSL.Util
 import Veil.SMT.Preparation
+import Veil.DSL.ActionLang
 
 open Lean Lean.Elab
 
@@ -46,5 +47,10 @@ def simplifyTerm (t : TSyntax `term) : TermElabM (TSyntax `term) := do
     -- definition, e.g. for transitions that are not actions.
     -- If that fails, we try to evaluate the term as is.
     -- We do `simp only [and_assoc]` at the end to normalize conjunctions.
-    first | (let t := conv! (dsimp only [$actSimp:ident]; simp only [$smtSimp:ident, $logicSimp:ident]; simp only [and_assoc]; simp only [↓ $elim_exists_State:ident]) => $t; exact t) | exact $t)
+    first | (let t := conv! (
+        dsimp only [$actSimp:ident];
+        unfold_wlp; dsimp only;
+        simp only [$smtSimp:ident, $logicSimp:ident];
+        simp only [and_assoc];
+        simp only [↓ $elim_exists_State:ident]) => $t; exact t) | exact $t)
   return t'
